$$
\displaystyle{\frac{\displaystyle{\frac{\displaystyle{\frac{\displaystyle{\frac{}{\neg (P \land Q),\;\neg (\neg P \lor \neg Q)\;\vdash \neg (P \land Q)}{\tiny\text{ax}}},\;\displaystyle{\frac{\displaystyle{\frac{\displaystyle{\frac{\displaystyle{\frac{\displaystyle{\frac{\displaystyle{\frac{\displaystyle{\frac{}{\neg (P \land Q),\;\neg (\neg P \lor \neg Q),\;P\;\vdash \neg (P \land Q)}{\tiny\text{ax}}},\;\displaystyle{\frac{\displaystyle{\frac{\displaystyle{\frac{\displaystyle{\frac{}{\neg (P \land Q),\;\neg (\neg P \lor \neg Q),\;P\;\vdash \neg (\neg P \lor \neg Q)}{\tiny\text{ax}}},\;\displaystyle{\frac{\displaystyle{\frac{\displaystyle{\frac{\displaystyle{\frac{}{\neg (P \land Q),\;\neg (\neg P \lor \neg Q),\;P,\;Q\;\vdash Q}{\tiny\text{ax}}},\;\displaystyle{\frac{\displaystyle{\frac{\displaystyle{\frac{}{\neg (P \land Q),\;\neg (\neg P \lor \neg Q),\;P,\;Q\;\vdash \neg (P \land Q)}{\tiny\text{ax}}},\;\displaystyle{\frac{\displaystyle{\frac{\displaystyle{\frac{}{\neg (P \land Q),\;\neg (\neg P \lor \neg Q),\;P,\;Q\;\vdash P}{\tiny\text{ax}}},\;\displaystyle{\frac{}{\neg (P \land Q),\;\neg (\neg P \lor \neg Q),\;P,\;Q\;\vdash Q}{\tiny\text{ax}}}}{\neg (P \land Q),\;\neg (\neg P \lor \neg Q),\;P,\;Q\;\vdash (P \land Q)}\wedge_i}}{\neg (P \land Q),\;\neg (\neg P \lor \neg Q),\;P,\;Q\;\vdash \neg \neg (P \land Q)}\textcolor{pink}{\neg\neg_i}}}{\neg (P \land Q),\;\neg (\neg P \lor \neg Q),\;P,\;Q\;\vdash \bot}\neg_e}}{\neg (P \land Q),\;\neg (\neg P \lor \neg Q),\;P,\;Q\;\vdash \neg Q}\neg_i}}{\neg (P \land Q),\;\neg (\neg P \lor \neg Q),\;P,\;Q\;\vdash \bot}\neg_e}}{\neg (P \land Q),\;\neg (\neg P \lor \neg Q),\;P\;\vdash \neg Q}\neg_i}}{\neg (P \land Q),\;\neg (\neg P \lor \neg Q),\;P\;\vdash \neg P \lor \neg Q}\vee_{i_2}}}{\neg (P \land Q),\;\neg (\neg P \lor \neg Q),\;P\;\vdash \bot}\neg_e}}{\neg (P \land Q),\;\neg (\neg P \lor \neg Q),\;P\;\vdash P \land Q}{\tiny\text{\textcolor{pink}{PBC}}}}}{\neg (P \land Q),\;\neg (\neg P \lor \neg Q),\;P\;\vdash \neg \neg (P \land Q)}\textcolor{pink}{\neg\neg_i}}}{\neg (P \land Q),\;\neg (\neg P \lor \neg Q),\;P\;\vdash \bot}\neg_e}}{\neg (P \land Q),\;\neg (\neg P \lor \neg Q),\;P\;\vdash \bot}\neg_i}}{\neg (P \land Q),\;\neg (\neg P \lor \neg Q)\;\vdash (\neg P \lor \neg Q)}\vee_{i_1}},\;\displaystyle{\frac{}{\neg (P \land Q),\;\neg (\neg P \lor \neg Q)\;\vdash \neg (\neg P \lor \neg Q)}{\tiny\text{ax}}}}{\neg (P \land Q),\;\neg (\neg P \lor \neg Q)\;\vdash \bot}\neg_e}}{\neg P \land Q,\;\neg (\neg P \lor \neg Q)\;\vdash (P \land Q)}{\tiny\text{\textcolor{pink}{PBC}}}}}{\neg (P \land Q),\;\neg (\neg P \lor \neg Q)\;\vdash \neg \neg (P \land Q)}\textcolor{pink}{\neg\neg_i}}}{\neg (P \land Q),\;\neg P \lor \neg Q\;\vdash \bot}\neg_e}}{\neg (P \land Q) \vdash \neg (\neg P \lor \neg Q)}{\tiny\text{\textcolor{pink}{PBC}}}}}{\neg (P \land Q) \Rightarrow \neg P \lor \neg Q}\Rightarrow_i}
$$