$$
\displaystyle{\frac{\displaystyle{\frac{\displaystyle{\frac{\displaystyle{\frac{}{\neg P \lor \neg Q,\;P \land Q\;\vdash \neg P \lor \neg Q}{\tiny\text{ax}}},\;\displaystyle{\frac{\displaystyle{\frac{}{\neg P \lor \neg Q,\;P \land Q\;\vdash \neg P \lor \neg Q}{\tiny\text{ax}}},\;\displaystyle{\frac{\displaystyle{\frac{\displaystyle{\frac{}{\neg P \lor \neg Q,\;P \land Q,\;\neg P\;\vdash \neg P}{\tiny\text{ax}}},\;\displaystyle{\frac{\displaystyle{\frac{}{\neg P \lor \neg Q,\;P \land Q,\;\neg P\;\vdash P \land Q}{\tiny\text{ax}}}}{\neg P \lor \neg Q,\;P \land Q,\;\neg P\;\vdash P}\wedge_{e_1}}}{\neg P \lor \neg Q,\;P \land Q,\;\neg P\;\vdash \bot}\neg_e}}{\neg P \lor \neg Q,\;P \land Q,\;\neg P\;\vdash \neg (\neg P \lor \neg Q)}\neg_i},\;\displaystyle{\frac{\displaystyle{\frac{\displaystyle{\frac{}{\neg P \lor \neg Q,\;P \land Q,\;\neg Q\;\vdash \neg Q}{\tiny\text{ax}}},\;\displaystyle{\frac{\displaystyle{\frac{}{\neg P \lor \neg Q,\;P \land Q,\;\neg Q\;\vdash P \land Q}{\tiny\text{ax}}}}{\neg P \lor \neg Q,\;P \land Q,\;\neg Q\;\vdash Q}\wedge_{e_1}}}{\neg P \lor \neg Q,\;P \land Q,\;\neg Q\;\vdash \bot}\neg_e}}{\neg P \lor \neg Q,\;P \land Q,\;\neg Q\;\vdash \neg (\neg P \lor \neg Q)}\neg_i}}{\neg P \lor \neg Q\;P \land Q \vdash \neg P \lor \neg Q}\neg_e}}{\neg P \lor \neg Q,\;P \land Q\;\vdash \bot}\neg_e}}{\neg P \lor \neg Q \vdash \neg (P \land Q)}\neg_i}}{\neg P \lor \neg Q \Rightarrow \neg (P \land Q)}\Rightarrow_i}
$$